@prefix xs: <http://www.w3.org/2001/XMLSchema#> .
@prefix skos: <http://www.w3.org/2004/02/skos/core#> .
@prefix rdf: <http://www.w3.org/1999/02/22-rdf-syntax-ns#> .
@prefix rdfs: <http://www.w3.org/2000/01/rdf-schema#> .
@prefix voc:	<http://visualartsdna.org/voc#> .

voc:visualArtsProcesses 
	a skos:ConceptScheme ;																									
	skos:prefLabel "visual arts processes" ;																				
	skos:hasTopConcept voc:process ;																									
	skos:definition "Processes are the steps taken to produce a completed creative work in the visual arts." ;
	skos:editorialNote "Care is taken to distinguish processes from techniques.  Processes focus on the order of steps while a technique can describe the details of a single step.  It is possible to conceive of a many-to-many relationship between processes and techniques depending on the scale at which each is defined." ;
	skos:note "Process is a useful concept but not a priority to elaborate on at this time." ;
	skos:notation "7d6563bf-305e-48d8-8ca8-00d5a5db1310" ;																									
.
																						
voc:visualArtsProcess																										
	a skos:Concept ;																									
	skos:prefLabel "visual arts process" ;																									
	skos:definition "A process used in the production of a creative work in the visual arts." ;			
	skos:notation "9d967b2a-009d-4a43-8028-24f8193f47c2" ;
	skos:inScheme voc:visualArtsProcesses ;																				
	.

voc:computerGraphicsProcesses 
	a skos:ConceptScheme ;																								
	skos:prefLabel "computer graphics processes" ;																				
	skos:hasTopConcept voc:computerGraphicsProcess ;																									
	skos:definition "The steps performed in the creation of a computer graphics creative work." ;
	skos:notation "dc9fb9b2-12c2-48a1-836a-ee473ca6581c" ;																									
.
																						
voc:computerGraphicsProcess																										
	a skos:Concept ;																									
	skos:prefLabel "computer graphics process" ;																									
	skos:broader voc:visualArtsProcess ;
	skos:definition "Computer graphics process is a step or set of steps performed in the creation of a computer graphics creative work." ;			
	skos:notation "ea834b4d-2362-4945-adb1-6c9eb5450e68" ;
	skos:inScheme voc:computerGraphicsProcesses ;																				
	.

voc:structuredDataGraphProcess																										
	a skos:Concept ;																									
	skos:prefLabel "structured data graph process" ;																									
	skos:broader voc:computerGraphicsProcess ;
	skos:definition "The process of producing a basic graphic representation of structured data." ;			
	skos:notation "1f4e2464-7a6d-4193-a784-33cd138cae4e" ;
	skos:inScheme voc:computerGraphicsProcesses ;																				
	.

voc:creativeGraphProcess																										
	a skos:Concept ;																									
	skos:prefLabel "creative graph process" ;																									
	skos:broader voc:computerGraphicsProcess ;
	skos:definition "The process of turning a graphic representation of structured data into a creative work." ;			
	skos:notation "0351dcb0-9697-46af-9ccd-278e0fed34a2" ;
	skos:inScheme voc:computerGraphicsProcesses ;																				
	.

voc:graphEmbellishmentProcess																										
	a skos:Concept ;																									
	skos:prefLabel "graph embellishment process" ;																									
	skos:broader voc:creativeGraphProcess ;
	skos:definition "Embellish a basic graphic representation of data." ;			
	skos:notation "2a4e80d9-5390-4c21-8607-02f95eb197a0" ;
	skos:inScheme voc:computerGraphicsProcesses ;																				
	.


voc:paintingProcesses 
	a skos:ConceptScheme ;																									
	skos:prefLabel "Painting processes" ;																				
	skos:hasTopConcept voc:paintingProcess ;																									
	skos:definition "Painting processes are the steps combining materials, techniques, tools and related concepts to produce a painting or to complete a part of the production of a painting." ;
	skos:notation "d36e4daf-1104-4dba-835c-17dbdf3ef3ea" ;																									
.
																						
voc:paintingProcess																										
	a skos:Concept ;																									
	skos:prefLabel "painting process" ;																									
	skos:broader voc:visualArtsProcess ;
	skos:definition "A process used in the production of a painting as a creative work." ;			
	skos:notation "88726b6d-d819-4280-9070-ad4d41d252d5" ;
	skos:inScheme voc:paintingTerms ;																				
	.

voc:paintingPostProduction
	a skos:Concept ;
	skos:prefLabel "painting post production" ;
	skos:broader voc:paintingProcess ;
	skos:definition "The process of removing ." ;
	skos:notation "45760261-2655-40c1-890c-2d21f57f5379" ;
	skos:inScheme voc:paintingProcesses ;																				
.

voc:paintingPreparation
	a skos:Concept ;
	skos:prefLabel "painting production" ;
	skos:broader voc:paintingProcess ;
	skos:definition "The process of creating a watercolor painting." ;
	skos:notation "48a09c53-3d5a-4d66-9bb3-fe055605573f" ;
	skos:inScheme voc:paintingProcesses ;																				
.

voc:painting
	a skos:Concept ;
	skos:prefLabel "painting" ;
	skos:broader voc:paintingProcess ;
	skos:definition "The process of creating a painting." ;
	skos:notation "1ab38e25-88c4-4a07-a9c7-303b5279ee0f" ;
	skos:inScheme voc:paintingProcesses ;																				
.

voc:substratePreparation
	a skos:Concept ;
	skos:prefLabel "substrate preparation" ;
	skos:broader voc:paintingPreparation ;
	skos:definition "The process of preparing the surface to receive the painting medium." ;
	skos:notation "e81d8cba-184a-4cbd-ae02-fa5ec9713c4e" ;
	skos:inScheme voc:paintingProcesses ;																				
.

voc:watercolorPaperPreparation
	a skos:Concept ;
	skos:prefLabel "watercolor paper preparation" ;
	skos:broader voc:substratePreparation ;
	skos:definition "The process of taping watercolor paper to a stable panel to support the paper during the application of watercolor painting techniques." ;
	skos:notation "d18d1a76-8afc-4239-9627-9a4b8905d93b" ;
	skos:inScheme voc:paintingProcesses ;																				
.

voc:watercolorPainting
	a skos:Concept ;
	skos:prefLabel "watercolor painting" ;
	skos:broader voc:paintingProcess ;
	skos:definition "The process of creating a watercolor painting." ;
	skos:notation "9238740c-dbd3-42e8-b292-22d07b3a25db" ;
	skos:inScheme voc:paintingProcesses ;																				
.


