@prefix xs: <http://www.w3.org/2001/XMLSchema#> .
@prefix skos: <http://www.w3.org/2004/02/skos/core#> .
@prefix rdf: <http://www.w3.org/1999/02/22-rdf-syntax-ns#> .
@prefix rdfs: <http://www.w3.org/2000/01/rdf-schema#> .
@prefix voc:	<http://visualartsdna.org/voc#> .

voc:watercolorPainting a skos:ConceptScheme ;																										
	skos:prefLabel "watercolor painting" ;																									
	skos:definition "Concepts in watercolor painting." ;																									
	skos:notation "67b6b185-d85b-4726-bfb5-288a4076a631" ;																									
	skos:inScheme voc:painting ;																				
	skos:hasTopConcept voc:watercolorTechnique ;																									
	skos:hasTopConcept voc:watercolorTerm ;																									
	skos:hasTopConcept voc:watercolorTool ;																									
	skos:hasTopConcept voc:watercolorMaterial ;																									
.																										
			
#voc:watercolorTechniques a skos:ConceptScheme ;																										
#	skos:hasTopConcept voc:watercolorTechnique ;																									
#	skos:prefLabel "watercolor painting techniques" ;																									
#	skos:definition "Techniques uses in watercolor painting." ;																									
#	skos:notation "5bd09167-7882-43fc-94b8-116a4681fe57" ;																									
#	skos:inScheme voc:watercolorPainting ;																				
#.																										
#			
#voc:watercolorTerms a skos:ConceptScheme ;																										
#	skos:hasTopConcept voc:watercolorTerm ;																									
#	skos:prefLabel "watercolor painting terms" ;																									
#	skos:definition "Terms used to describe the art of watercolor painting." ;																									
#	skos:notation "f655ef38-987c-4486-b693-1a8199952c50" ;																									
#	skos:inScheme voc:watercolorPainting ;																				
#.																										
#			
#voc:watercolorTools a skos:ConceptScheme ;																										
#	skos:hasTopConcept voc:watercolorTool ;																									
#	skos:prefLabel "watercolor painting tools" ;																									
#	skos:definition "Tools used in watercolor painting." ;																									
#	skos:notation "266557ff-2fe5-4324-92e0-693ad761ad6c" ;																									
#	skos:inScheme voc:watercolorPainting ;																				
#.																										
#			
#voc:watercolorMaterials a skos:ConceptScheme ;																										
#	skos:hasTopConcept voc:watercolorMaterial ;																									
#	skos:prefLabel "watercolor materials" ;																									
#	skos:definition "Materials used in watercolor painting." ;																									
#	skos:notation "ee38b38c-62af-42ab-92a0-7a2c1ec3b21d" ;																									
#	skos:inScheme voc:watercolorPainting ;																				
#.																										
			
# top concepts																							
voc:watercolorTechnique																										
	a skos:Concept ;																									
	skos:prefLabel "watercolor technique" ;																									
	skos:broader voc:paintingTechnique ;
	skos:definition "A technique used in watercolor painting." ;			
	skos:notation "08477a20-cbf0-4937-a1fe-bf40e7442b83" ;
	skos:inScheme voc:watercolorPainting ;																				
	.
voc:watercolorTerm																										
	a skos:Concept ;																									
	skos:prefLabel "watercolor term" ;																									
	skos:broader voc:paintingTerm ;
	skos:definition "A term of art in watercolor painting." ;																									
	skos:notation "4d7f39c2-544b-47a8-b04f-f656a58c608d" ;
	skos:inScheme voc:watercolorPainting ;																				
	.
voc:watercolorMaterial																										
	a skos:Concept ;																									
	skos:prefLabel "watercolor material" ;																									
	skos:broader voc:paintingMaterial ;
	skos:definition "A material used in watercolor painting." ;																									
	skos:notation "24eb6db8-cef8-4ff8-9d68-8529aec6cf00" ;
	skos:inScheme voc:watercolorPainting ;																				
	.
voc:watercolorTool																										
	a skos:Concept ;																									
	skos:prefLabel "watercolor tool" ;																									
	skos:definition "A tool used in watercolor painting." ;																									
	skos:broader voc:paintingTool ;
	skos:notation "24eb6db8-cef8-4ff8-9d68-8529aec6cf00" ;
	skos:inScheme voc:watercolorPainting ;																				
	.

# hierarchical terms
voc:diffusingPaint
	a skos:Concept ;
	skos:prefLabel "paint diffusion" ;
	skos:broader voc:watercolorTechnique ;
	skos:definition "To spread over an area with paint in an aerosol form." ;
	skos:notation "1ffac74d-9b0c-4811-b28d-f39a6b780a14" ;
	skos:inScheme voc:watercolorPainting ;																				
	.

voc:removingPaint
	a skos:Concept ;
	skos:prefLabel "removing paint" ;
	skos:broader voc:watercolorTechnique ;
	skos:definition "The removal of paint with a tool." ;
	skos:notation "8952c9fd-3458-4ce0-a3c1-542cc50e2879" ;
	skos:inScheme voc:watercolorPainting ;																				
	.

voc:inkWash
	a skos:Concept ;
	skos:prefLabel "ink wash" ;
	skos:broader voc:wetIntoWetWash ;
	skos:definition "A watercolor wash of ink." ;
	skos:notation "ab877d65-1983-40df-9587-f4ebea7c8751" ;
	skos:inScheme voc:watercolorPainting ;																				
	.

voc:assistedWash
	a skos:Concept ;
	skos:prefLabel "assisted wash" ;
	skos:broader voc:wetIntoWetWash ;
	skos:definition "A watercolor wash in the presence of another material intended to affect the behavior of the wash." ;
	skos:notation "4428e7ab-1b5e-4e34-a10f-0ca72bfca245" ;
	skos:inScheme voc:watercolorPainting ;																				
	.


# collected terms


voc:atomiserSprayer
	a skos:Concept ;
	skos:prefLabel "atomiser sprayer" ;
	skos:related voc:atomiser ;
	skos:broader voc:watercolorTool ;
	skos:definition "Manual (mouth operated) paint spraying tool that creates a fine mist and similar painting effect to an airbrush or aerosol spray can; sometimes referred to as a diffuser." ;
	skos:notation "4840175c-0801-4b1d-b70d-796a9dfe71c8" ;
	skos:inScheme voc:watercolorPainting ;																				
	.

voc:atomiser
	a skos:Concept ;
	skos:prefLabel "atomiser" ;
	skos:broader voc:diffusingPaint ;
	skos:definition "The process of spraying a fine mist, similar painting effect to an airbrush or aerosol spray can; sometimes referred to as a diffuser." ;
	skos:notation "ff3bbde9-61c3-4c15-92cc-82b3c3de1354" ;
	skos:inScheme voc:watercolorPainting ;																				
	.


voc:backrun
	a skos:Concept ;
	skos:prefLabel "backrun" ;
	skos:altLabel "Back Run" ;
	skos:broader voc:wetIntoWetWash ;
	skos:editorialNote "The mixing of colours in a semi-controlled way by adding new colour to a wash that hasn't dried; backruns can be an unwelcome accident, but are also deliberately created by some artists to represent abstracted clouds, foliage or flowers, or just to create a specific mood and for visual interest." ;
	skos:definition "A back run occurs when painting into a wet area of watercolor with a mix of paint that is more dilute than is currently there. This causes the paint to spread out (Bloom) and often leaves a cauliflower shaped pattern when dry. This is often considered to be undesirable but can also be done intentionally to create a textural effect." ;
	skos:notation "08ca18e5-e300-4a0b-b2cb-9d8f35865db0" ;
	skos:inScheme voc:watercolorPainting ;																				
	.


voc:bambooBrush
	a skos:Concept ;
	skos:prefLabel "bamboo brush" ;
	skos:broader voc:watercolorTool ;
	skos:definition "An inexpensive natural haired chinese style brush (Often squirrel hair) that has a bamboo handle and is mainly used to create loose painterly strokes.I love using this brush for natural looking foliage and skiesI love using this brush for natural looking foliage and skies" ;
	skos:notation "97bbc4a6-b170-4bd5-a44a-1a9e71bcd0a3" ;
	skos:inScheme voc:watercolorPainting ;																				
	.


voc:bead
	a skos:Concept ;
	skos:prefLabel "bead" ;
	skos:broader voc:wash ;
	skos:definition "A bead is the line of water that pools at the base of a Wash. Maintaining the bead becomes important when attempting to paint a consistent wash as streaks will occur in the if it dries out too quickly." ;
	skos:notation "fc4fb13c-8ec0-4baf-9643-cf839f6aa0d4" ;
	skos:inScheme voc:watercolorPainting ;																				
	.


voc:binder
	a skos:Concept ;
	skos:prefLabel "binder" ;
	skos:broader voc:watercolorMaterial ;
	skos:definition "Binder is a substance that holds watercolor pigment in suspension. The substance used is generally Gum Arabic or synthetic Glycol." ;
	skos:notation "72ebc54c-a920-43a9-8167-fdef3ec766eb" ;
	skos:inScheme voc:watercolorPainting ;																				
	.


voc:block
	a skos:Concept ;
	skos:prefLabel "block" ;
	skos:broader voc:watercolorMaterial ;
	skos:definition "Watercolor paper is often sold in a “Block”, which is a number of sheets of paper that are glued around the edges as opposed to loose. This minimizes Cockling and eliminates the need for stretching paper." ;
	skos:notation "dfbfbed8-5f4b-42e8-b4fe-d6a71882ff9e" ;
	skos:inScheme voc:watercolorPainting ;																				
	.


voc:bloom
	a skos:Concept ;
	skos:prefLabel "bloom" ;
	skos:broader voc:watercolorTechnique ;
	skos:definition "See Backrun" ;
	skos:notation "243e9a3e-e5db-4de4-8ada-104e21b65d28" ;
	skos:inScheme voc:watercolorPainting ;																				
	.


voc:blottingPapper
	a skos:Concept ;
	skos:prefLabel "blotting paper" ;
	skos:broader voc:watercolorMaterial ;
	skos:definition "Paper type; Blotter paper; a highly absorbent type of paper used to absorb an excess of liquid (such as ink or paint) from the substrate." ;
	skos:notation "3f563b12-2a7e-44f2-86bc-2ecb751c08f9" ;
	skos:inScheme voc:watercolorPainting ;																				
	.


voc:bodyColour
	a skos:Concept ;
	skos:prefLabel "body colour" ;
	skos:broader voc:watercolorMaterial ;
	skos:definition "Paint type; a slightly confusing term that simply means opaque water-based paint (such as Gouache or Tempera). Opaque colours can be used to add punches of solid colour to transparent watercolours, and opaque white is used to bring highlights back out of muddy or over-saturated areas." ;
	skos:notation "06816e3d-ccaa-453e-954b-d2bc1e840cf8" ;
	skos:inScheme voc:watercolorPainting ;																				
	.


voc:buckle
	a skos:Concept ;
	skos:prefLabel "buckle" ;
	skos:broader voc:watercolorTerm ;
	skos:definition "wavy, uneven surface once water has been applied; can and should be avoided by stretching the paper prior to painting. (see; stretching)Although some aspects of painting once thought to be negative (such as backruns) can be used to ones advantage, buckling paper is never desired and never considered a happy accident." ;
	skos:notation "7d7a7228-2199-46af-b6c2-c39747b0e6c9" ;
	skos:inScheme voc:watercolorPainting ;																				
	.


voc:watercolorCanvas
	a skos:Concept ;
	skos:prefLabel "canvas" ;
	skos:broader voc:canvas ;
	skos:definition "Watercolor canvas is similar to oil painting canvas. Watercolor canvas has been treated with Gesso to enable it to take water based paints." ;
	skos:notation "ea6b1e7e-672b-4063-ba59-89d7cd3c0a09" ;
	skos:inScheme voc:watercolorPainting ;																				
	.


voc:casein
	a skos:Concept ;
	skos:prefLabel "casein" ;
	skos:broader voc:watercolorMaterial ;
	skos:definition "Casein is a water based painting medium derived from milk. It’s properties resemble Gouache. A fast-drying, water-soluble paint derived from milk protein, or casein" ;
	skos:notation "e9758c98-3e7b-44d1-8bc5-12da4e8d6a72" ;
	skos:inScheme voc:watercolorPainting ;																				
	.




voc:catsTongue
	a skos:Concept ;
	skos:prefLabel "cat's tongue" ;
	skos:broader voc:watercolorTool ;
	skos:definition "Brush type; similar in shape to a Filbert brush, but with a pointed tip. The ideal tool for creating single-stroke flower petals and leaves.To help clarify the definitions of specialty brushes in this glossary, use this visual guide to basic brush shapes as a reference." ;
	skos:notation "b084ec7a-bef0-4fc0-a9a8-b37e419aadbd" ;
	skos:inScheme voc:watercolorPainting ;																				
	.


voc:cauliflower
	a skos:Concept ;
	skos:prefLabel "cauliflower" ;
	skos:broader voc:watercolorTerm ;
	skos:definition "(See Backrun)" ;
	skos:notation "698a5086-a2ac-4817-bf23-0eb5372efff5" ;
	skos:inScheme voc:watercolorPainting ;																				
	.


voc:charging
	a skos:Concept ;
	skos:prefLabel "charging" ;
	skos:broader voc:wetIntoWetWash ;
	skos:definition "Is a technique that involves dropping a new wet color into an existing wash allowing them to blend ad create interesting variations of color or tonal value. Mixing two or more colors directly on the paper instead of premixing on a palette" ;	skos:notation "2aa59820-ad46-40f3-a929-bfd694017a7d" ;
	skos:inScheme voc:watercolorPainting ;																				
	.


voc:cockling
	a skos:Concept ;
	skos:prefLabel "cockling" ;
	skos:broader voc:watercolorTerm ;
	skos:definition "Cockling, or buckling, occurs when a sheet of watercolor paper is wet. This creates a series of uneven undulations or ridges which can cause problems when trying to paint. Cockling can be minimized by Stretching, using heavier Weight paper such as 140lb/300gsm or above, or by using a watercolor Block." ;
	skos:notation "1c58fc88-760f-463c-8502-9b75a7dfe897" ;
	skos:inScheme voc:watercolorPainting ;																				
	.


voc:coldPressedPaper
	a skos:Concept ;
	skos:prefLabel "cold-pressed paper" ;
	skos:altLabel "Cold Pressed" ;
	skos:broader voc:watercolorMaterial ;
	skos:definition "The most commonly used type of watercolour paper; a heavy weight; absorbent paper featuring a pronounced toothy finish and sized to accept watermedia (see; sizing).Highest quality cold pressed papers may be hand-made and will contain 100% cotton fibres; they're loved for their irregular rough texture and reliable performance and absorbency" ;	skos:notation "1da470ac-6388-4c5a-917a-7d45bd4bd621" ;
	skos:inScheme voc:watercolorPainting ;																				
	.


voc:daggerBrush
	a skos:Concept ;
	skos:prefLabel "dagger brush" ;
	skos:broader voc:watercolorTool ;
	skos:definition "A dagger brush has a straight edge and a sloping edge reminiscent of a knife blade. This brush is ideal for painting thin or tapering lines." ;
	skos:notation "ec05534b-fa30-4f4e-8b49-b89800a76de2" ;
	skos:inScheme voc:watercolorPainting ;																				
	.


voc:deckledEdges
	a skos:Concept ;
	skos:prefLabel "deckled edges" ;
	skos:broader voc:watercolorTerm ;
	skos:definition "This refers to the rough untrimmed edges of certain brands of watercolor paper." ;
	skos:notation "fe497cf9-3d45-4f28-a7ca-31f4881ba1af" ;
	skos:inScheme voc:watercolorPainting ;																				
	.


voc:watercolorEasel
	a skos:Concept ;
	skos:prefLabel "easel" ;
	skos:broader voc:easel ;
	skos:definition "A stable stand, with an angled board that supports an artist’s painting ." ;
	skos:notation "606c5824-1ddc-405d-ad14-3c669e2c4ed5" ;
	skos:inScheme voc:watercolorPainting ;																				
	.


voc:fanBrush
	a skos:Concept ;
	skos:prefLabel "fan brush" ;
	skos:altLabel "Fan" ;
	skos:broader voc:watercolorTool ;
	skos:definition "A fan brush is often used in watercolor painting for painting grass and foliage. It is a short haired brush with the hairs spread out out in a fan shape.  Ideal for blending edges, or mimicking the texture of many things such as fur, feathers, ripples on water, grasses, tree boughs." ;
	skos:notation "9cd8b9a5-274a-405f-93f1-f907596330ac" ;
	skos:inScheme voc:watercolorPainting ;																				
	.


voc:flatBrush
	a skos:Concept ;
	skos:prefLabel "flat brush" ;
	skos:broader voc:watercolorTool ;
	skos:definition "A flat brush is a short haired brush with a straight edge. Flat brushes are generally useful for laying down washes of all kinds and are particularly useful for painting hard edged shapes such as mountains tree trunks etc.Great for crisp hard edges, washes, buildings and figuresGreat for crisp hard edges, washes, buildings and figures" ;
	skos:notation "498e3dcb-872c-4590-a250-a8927b625a2a" ;
	skos:inScheme voc:watercolorPainting ;																				
	.


voc:flatWash
	a skos:Concept ;
	skos:prefLabel "flat wash" ;
	skos:broader voc:wetOnDry ;
	skos:definition "brushing successive strokes of color on a wet or dry surface, with each stroke placed next to the other, to create an even layer of color" ;
	skos:notation "6a6a55eb-0043-4f92-a4d6-0a70b220639d" ;
	skos:inScheme voc:watercolorPainting ;																				
	.


voc:frisket
	a skos:Concept ;
	skos:prefLabel "frisket" ;
	skos:broader voc:watercolorTool ;
	skos:editorialNote "This could be considered a material, as well" ;
	skos:definition "A fluid composition of liquid latex and ammonia, or an adhesive film; used to cover (mask-off) areas of of your painting where paint is not wanted; excellent at preserving white space. (see; masking, white space)Liquid frisket dries very quickly and can be easily peeled off waterclour paper (or rubbed off with an eraser) when no longer needed. Frisket adhesive film must be cut to shape and then applied to the paper; the low tack of the adhesive film allows it to be easily removed when no longer needed." ;
	skos:notation "d6ecf650-7942-4c82-aa6a-0ffc3e4f6b77" ;
	skos:inScheme voc:watercolorPainting ;																				
	.


voc:watercolorGlazing
	a skos:Concept ;
	skos:prefLabel "glazing" ;
	skos:altLabel "layering" ;
	skos:broader voc:wetOnDry ;
	skos:definition "Glazing, or layering, is the technique of laying a thin wash of color over the top of another color which has dried. Due to the transparency of watercolor, this can have he effect of creating a third color or can simply be used to darken an existing color." ;
	skos:notation "9e23366d-aba2-4e26-9802-7cf15a9539f2" ;
	skos:inScheme voc:watercolorPainting ;																				
	.


voc:gouache
	a skos:Concept ;
	skos:prefLabel "gouache" ;
	skos:altLabel "gouache (or body color)" ;
	skos:broader voc:watercolorMaterial ;
	skos:definition "Gouache is similar to watercolor but is much more opaque.  An opaque watercolor that can be applied thick or thin" ;
	skos:notation "94e719bd-d7c1-4b00-8dfa-a4583495db47" ;
	skos:inScheme voc:watercolorPainting ;																				
	.


voc:gradatedWash
	a skos:Concept ;
	skos:prefLabel "gradated wash" ;
	skos:broader voc:wetIntoWetWash ;
	skos:definition "A wash in which the value  gradually changes from dark to light.  A graduated wash is painted like a flat wash except that more water is added incrementally to lighten the colour as the wash progresses. This technique can be useful for painting skies and seas etc." ;
	skos:notation "3f74ecee-8045-40f3-a1a7-4911cf72fbc2" ;
	skos:inScheme voc:watercolorPainting ;																				
	.


voc:granulation
	a skos:Concept ;
	skos:prefLabel "granulation" ;
	skos:altLabel "Granulating" ;
	skos:broader voc:watercolorTerm ;
	skos:definition "The tendency for some colour pigments to precipitate (or settle out) when water is added, resulting in a granular, speckled effect; also commonly referred to as sedimentary colours; it's a natural effect, not indicative of poor quality paint, or technical misuse. Only some colours will granulate." ;
	skos:notation "3e28fb76-7641-4853-8c4f-9d7eb54ea84e" ;
	skos:inScheme voc:watercolorPainting ;																				
	.


voc:watercolorGround
	a skos:Concept ;
	skos:prefLabel "ground" ;
	skos:broader voc:watercolorMaterial ;
	skos:definition "Watercolor ground is an acrylic based primer that allows a degree of absorbency. This enables a watercolor artist to paint on surfaces which would not usually be suitable for watercolor paint such as printer paper, thin card or even materials such as wood or stone." ;
	skos:notation "b7818ea2-e446-422b-9ab2-68f512be6c20" ;
	skos:inScheme voc:watercolorPainting ;																				
	.


voc:gumArabic
	a skos:Concept ;
	skos:prefLabel "gum arabic" ;
	skos:broader voc:watercolorMaterial ;
	skos:definition "A natural non-toxic gum made from the sap of various species of the acacia tree used as a binder in watercolours; gum arabic fluid can be added to colours to thicken inks and watercolours, increasing the viscosity of the paint film and also intensifying colours. Gum arabic can also be diluted with water and applied directly to watercolour paper as a sealant, making it less absorbent, or over top of a finished watercolour painting (much like a varnish)." ;
	skos:notation "f9674a0f-f8f4-41ea-ba02-33c68af68357" ;
	skos:inScheme voc:watercolorPainting ;																				
	.


voc:hakeBrush
	a skos:Concept ;
	skos:prefLabel "hake brush" ;
	skos:broader voc:watercolorTool ;
	skos:definition "The Hake is a traditional wide short-haired, long-handled Japanese brush into which goat’s hair is stitched. The Hake brush is useful for painting natural looking foliage and skies. It was popularized by artist/author Ron Ranson." ;
	skos:notation "fd5ed5b4-d6a0-4569-b558-e9d9afb0732d" ;
	skos:inScheme voc:watercolorPainting ;																				
	.


voc:happyAccident
	a skos:Concept ;
	skos:prefLabel "happy accident" ;
	skos:broader voc:watercolorTerm ;
	skos:editorialNote "This better belongs under paintingTerm when that is available" ;
	skos:definition "An unintended and unforeseen event that occurred during the course of a painting which nevertheless resulted in a desirable effect." ;
	skos:notation "08b8c08d-0c6b-498d-afd7-fa36f2f7835d" ;
	skos:inScheme voc:watercolorPainting ;																				
	.


voc:hardEdge
	a skos:Concept ;
	skos:prefLabel "hard edge" ;
	skos:broader voc:watercolorTerm ;
	skos:definition "The edge of a shape that is sharply defined, as opposed to Soft Edge." ;
	skos:notation "aac9dd1b-e104-42b4-ba07-f5f7c101cf98" ;
	skos:inScheme voc:watercolorPainting ;																				
	.


voc:hotPressedPaper
	a skos:Concept ;
	skos:prefLabel "hot pressed paper" ;
	skos:altLabel "Hot Pressed" ;
	skos:broader voc:watercolorMaterial ;
	skos:definition "Paper type; a heavy-weight, slow-to-absorb paper featuring a very smooth finish; manufactured using steam, heat and/or pressure to to help the fibres (wood pulp and/or cotton) nestle very close together, making the paper very slow to absorb; sized for water media." ;
	skos:notation "f5de000a-e1d7-4513-a493-2ccfd0e1ac90" ;
	skos:inScheme voc:watercolorPainting ;																				
	.



voc:impressing
	a skos:Concept ;
	skos:prefLabel "impressing" ;
	skos:broader voc:watercolorTechnique ;
	skos:definition "Pressing plastic wrap or fabric into a still wet application of paint; capable of creating a vast array textured effects." ;
	skos:notation "3408ef21-a909-48e2-8864-7b8fb1e2a3b3" ;
	skos:inScheme voc:watercolorPainting ;																				
	.


voc:indenting
	a skos:Concept ;
	skos:prefLabel "indenting" ;
	skos:broader voc:watercolorTechnique ;
	skos:definition "Scoring the paper (using a stylus or the end of a paintbrush) directly after an application of fresh paint; the scored marks are recessed into the paper so pigments will naturally settle in the lines, showing off the scored details." ;
	skos:notation "a09a992c-c6b9-456e-8989-503e5c4f1036" ;
	skos:inScheme voc:watercolorPainting ;																				
	.


voc:kolinskySable
	a skos:Concept ;
	skos:prefLabel "Kolinsky (sable)" ;
	skos:broader voc:watercolorTool ;
	skos:definition "Is a species of weasel found in Siberia. The most highly prized and expensive watercolor brushes are made from the tail hairs of the male of the species." ;
	skos:notation "b0b551d4-475f-49a0-9db1-04537b0c4c9f" ;
	skos:inScheme voc:watercolorPainting ;																				
	.


voc:liftingPaint
	a skos:Concept ;
	skos:prefLabel "lifting paint" ;
	skos:altLabel "Lifting" ;
	skos:altLabel "Lifting Out" ;
	skos:broader voc:removingPaint ;
	skos:definition "Removing paint from a surface with a brush, paper towel or tissue. Removing colour from an area of wet paint, or re-wetting an area of dried paint and removing colour; a painting technique in it's own right, not just a correction method; the basis of subtractive painting.Lifting creates soft edges and can diffuse or modify colours, reducing their intensity and leaving only the undertones. Strategic or detailed lifts can be done using a slightly damp paintbrush to wick up the colour." ;
	skos:notation "8eb58275-7d2a-4111-b087-5bbb31aad7cf" ;
	skos:inScheme voc:watercolorPainting ;																				
	.


voc:lineWash
	a skos:Concept ;
	skos:prefLabel "line & wash" ;
	skos:broader voc:inkWash ;
	skos:definition "Line and wash is the technique of combining ink pen drawings with with watercolors. Traditionally this was done with dip pens but can also be done with markers, biros and Rapidograph style engineering drawing pens." ;
	skos:notation "36bdab9b-7f8c-40a9-8338-c8c39b02e1b3" ;
	skos:inScheme voc:watercolorPainting ;																				
	.


voc:linerRigger
	a skos:Concept ;
	skos:prefLabel "liner rigger" ;
	skos:broader voc:watercolorTool ;
	skos:definition "Brush type; similar in shape to round brushes but with hairs that are twice the usual length; ideal for drawing out long, thin continuous lines; available in small sizes only (#3 is generally the largest size).It's debatable whether there's any difference between Liners and Riggers. Brush manufacturers don't seem to differentiate; one will call it a rigger, while the other calls it a liner, yet the brush is identical for all intents and purposes.x" ;
	skos:notation "42ae1e44-6749-44d6-a5cf-3241cae0b967" ;
	skos:inScheme voc:watercolorPainting ;																				
	.


voc:loosePaintingStyle
	a skos:Concept ;
	skos:prefLabel "loose painting style" ;
	skos:broader voc:watercolorTechnique ;
	skos:definition "The loose painting style is characterized by a quick and impressionistic approach to painting. Many watercolor artists love to work in this style because of it’s spontaneous and lively appearance." ;
	skos:example <https://www.youtube.com/watch?v=AWtjbE84XGI> ;
	skos:editorialNote "This video seems the epitome of loose painting style" ;
	skos:notation "1713297c-7c97-4506-a4ec-07b681c93c88" ;
	skos:inScheme voc:watercolorPainting ;																				
	.


voc:lostAndFoundEdges
	a skos:Concept ;
	skos:prefLabel "lost and found edges" ;
	skos:altLabel "Lost & Found Edges" ;
	skos:broader voc:watercolorTechnique ;
	skos:definition "When the tonal value of the edge of a foreground object begins to matches the tonal value of it’s background the edges of the object start to become indiscernible against the background. This creates the appearance the optical illusion of a disappearing edge but the brain still interprets the edge as being present. This is often used to create a deliberate effect, used to create and suggest movement. A found edge is the reversal of this." ;
	skos:notation "228946c0-dd45-45ce-9a92-b665abc19581" ;
	skos:inScheme voc:watercolorPainting ;																				
	.

voc:masking
	a skos:Concept ;
	skos:prefLabel "masking" ;
	skos:broader voc:assistedWash ;
	skos:editorialNote "Chose to use 'masking' for the technique and 'maskingFluid' for the material; however, 'masking' does not necessarily imply the use of masking fluid" ;
	skos:definition "In watercolor painting, white areas are usually depicted by preserving the white of the paper. Masking fluid is a rubbery fluid which can be painted on to the watercolor paper and once dry, can be painted over preventing water from seeping through on to the paper. Masking fluid can be removed with gentle rubbing and peeling once the paint is dry." ;
	skos:notation "bea51728-f85f-4861-b0bf-c1374b2ef92d" ;
	skos:inScheme voc:watercolorPainting ;																				
	.

voc:maskingFluid
	a skos:Concept ;
	skos:prefLabel "masking Fluid" ;
	skos:broader voc:watercolorMaterial ;
	skos:related voc:masking ;
	skos:definition "Liquid latex used to preserve the white of the paper and to create textures" ;
	skos:notation "d51e34e0-881c-4802-89ba-a694491ead7c" ;
	skos:inScheme voc:watercolorPainting ;																				
	.


voc:watercolorMedium
	a skos:Concept ;
	skos:prefLabel "watercolor medium" ;
	skos:broader voc:watercolorMaterial ;
	skos:definition "Watercolor medium is a substance which can be added to watercolor paint to create effects that couldn’t be obtained purely with water, such as texture, gloss or glitter." ;
	skos:notation "a2d90dab-799f-4a1d-9506-08b03750395d" ;
	skos:inScheme voc:watercolorPainting ;																				
	.


voc:mopBrush
	a skos:Concept ;
	skos:prefLabel "mop brush" ;
	skos:altLabel "Mop" ;
	skos:broader voc:watercolorTool ;
	skos:definition "A mop brush is a type of Round Brush that has a thick hair at it’s base tapering into a very thin tip. The mop brush is very versatile and can create many different kinds of strokes." ;
	skos:notation "05d5169b-db58-4180-bca2-7e36edab84a8" ;
	skos:inScheme voc:watercolorPainting ;																				
	.


voc:mud
	a skos:Concept ;
	skos:prefLabel "mud" ;
	skos:broader voc:watercolorTerm ;
	skos:definition "Mud refers to the dull earthy neutral colors that result from mixing colors that contain too much of their complementary hue. e.g mixing a red with a green." ;
	skos:notation "22949d4e-a4bd-4df1-9ad2-5e3d7ac2cae0" ;
	skos:inScheme voc:watercolorPainting ;																				
	.


voc:notPaper
	a skos:Concept ;
	skos:prefLabel "not paper" ;
	skos:broader voc:watercolorMaterial ;
	skos:definition "Is the British convention for referring to Cold Pressed watercolor paper, it simply means “Not hot pressed”" ;
	skos:notation "65518f69-0a14-4b57-a329-f7d76d2acb3e" ;
	skos:inScheme voc:watercolorPainting ;																				
	.


voc:naturalHairBrushes
	a skos:Concept ;
	skos:prefLabel "natural hair brushes" ;
	skos:broader voc:watercolorTool ;
	skos:definition "Brushes that contain animal hair such as squirrel, sable or goat" ;
	skos:notation "31cf91de-5a5a-4152-80d9-483ea3345bd7" ;
	skos:inScheme voc:watercolorPainting ;																				
	.



voc:overPainting
	a skos:Concept ;
	skos:prefLabel "over-painting" ;
	skos:broader voc:brushingPaint ;
	skos:definition "Cleaning up muddy or over-saturated areas, restoring white space (see; white space), creating highlights, or making blurry edges crisp again; generally speaking, over-painting is done with an opaque white water-based paint (such as Titanium White Gouache, or Chinese White Watercolour).Some traditionalist folks consider over-painting to be cheating, however it's a widely practiced technique and can be artfully done.  Over-painting is often a much better solution than chucking out an otherwise successful painting.... Besides, who cares what some folks think! Art is not meant to be perfection." ;
	skos:notation "b532d2eb-1a7c-463c-b670-d61a34013c85" ;
	skos:inScheme voc:watercolorPainting ;																				
	.


voc:overworking
	a skos:Concept ;
	skos:prefLabel "overworking" ;
	skos:broader voc:watercolorTerm ;
	skos:definition "This occurs when you carry on adding more and more to a painting when it would have been stopping at an earlier stage would have resulted in a livelier fresher looking piece of work. This is rather subjective and can be difficult to judge. Try and evaluate what you’re trying to achieve with every single brushstroke before making it rather than just mindlessly piling on more." ;
	skos:notation "043a3cf1-c5aa-4e4c-b410-685b8173cee0" ;
	skos:inScheme voc:watercolorPainting ;																				
	.


voc:oxGall
	a skos:Concept ;
	skos:prefLabel "ox gall" ;
	skos:broader voc:watercolorMaterial ;
	skos:definition "Yellowish fluid from gall bladders (usually obtained from cows) mixed with alcohol and used as the wetting agent in paper marbling and watercolor painting.If a watercolour wash is not covering the paper evenly, is beading up, or failing to absorb into the deep texture of the paper leaving tiny white specks, add a drop of ox gall to improve flow and even out the absorbancy." ;
	skos:notation "46ca71f1-9c15-4c35-ac6b-07851853ede2" ;
	skos:inScheme voc:watercolorPainting ;																				
	.

voc:panPaint
	a skos:Concept ;
	skos:prefLabel "pan paint" ;
	skos:broader voc:watercolorMaterial ;
	skos:definition "small cakes of watercolor paint that come in half-pan or whole-pan sizes" ;
	skos:notation "e0fde960-13c1-4ba1-a212-569e6c0c2307" ;
	skos:inScheme voc:watercolorPainting ;																				
	.


voc:pan
	a skos:Concept ;
	skos:prefLabel "pan" ;
	skos:broader voc:watercolorTool ;
	skos:definition "Pans are small thumbnail sized paint containers that slot into portable trays. Pans are most often used for painting in small sketchbooks and outdoors" ;
	skos:notation "b63c1c11-8d41-499a-aad3-b3a2ce83b52a" ;
	skos:inScheme voc:watercolorPainting ;																				
	.


voc:resist
	a skos:Concept ;
	skos:prefLabel "resist" ;
	skos:broader voc:assistedWash ;
	skos:definition "Any substance that can be applied to watercolour paper that will repel water and therefore paint pigment as well; wax crayons and oil pastels are commonly used resists: resists are generally a permanent addition to your painting (unlike frisket which is removed)." ;
	skos:notation "9ca85d90-be59-4150-8d1d-88bf707e8103" ;
	skos:inScheme voc:watercolorPainting ;																				
	.


voc:rigger
	a skos:Concept ;
	skos:prefLabel "rigger" ;
	skos:broader voc:watercolorTool ;
	skos:definition "A rigger is a watercolour brush with long thin hairs. It is useful for painting thin lines such as the rigging on ships, hence the name." ;
	skos:notation "c2cd5b73-f103-466a-9cb0-23ad54508f83" ;
	skos:inScheme voc:watercolorPainting ;																				
	.


voc:roughPaper
	a skos:Concept ;
	skos:prefLabel "rough paper" ;
	skos:broader voc:watercolorMaterial ;
	skos:definition "Heavily textured watercolor paper" ;
	skos:notation "4994d844-b6f8-41a6-afdf-d2979179b582" ;
	skos:inScheme voc:watercolorPainting ;																				
	.


voc:roundBrush
	a skos:Concept ;
	skos:prefLabel "round brush" ;
	skos:broader voc:watercolorTool ;
	skos:definition "A very commonly used watercolor brush with hairs that taper to a fine point. The round brush is a versatile brush that can be used to paint a variety of brush strokes.A very versatile brush. It can be used for painting washes, fine details and broad strokes" ;
	skos:notation "ccf11591-7c8d-4bc5-b986-b5b2b7428482" ;
	skos:inScheme voc:watercolorPainting ;																				
	.


voc:sandingDryPaper
	a skos:Concept ;
	skos:prefLabel "sanding dry paper" ;
	skos:broader voc:removingPaint ;
	skos:definition "Unusual textures can be made by lightly sanding the surface of a very dry painting with fine sandpaper. The surface takes on a slightly weathered appearance. The sanded area can be adjusted by the application of further washes." ;
	skos:notation "103dd0d3-2804-408e-b22f-448f1cae569f" ;
	skos:inScheme voc:watercolorPainting ;																				
	.


voc:scrubbing
	a skos:Concept ;
	skos:prefLabel "scrubbing" ;
	skos:broader voc:removingPaint ;
	skos:definition "A dry brush technique used to lift paint from or add color to an area of the surface" ;
	skos:notation "1a96f4f6-64bf-4a64-bd7e-b0ff531579fe" ;
	skos:inScheme voc:watercolorPainting ;																				
	.


voc:sedimentary
	a skos:Concept ;
	skos:prefLabel "sedimentary" ;
	skos:broader voc:watercolorTerm ;
	skos:definition "Paint characteristic; see granulation" ;
	skos:notation "b376c03a-09f0-4252-8bd6-b8126d8a7f20" ;
	skos:inScheme voc:watercolorPainting ;																				
	.


voc:shader
	a skos:Concept ;
	skos:prefLabel "shader" ;
	skos:broader voc:watercolorTool ;
	skos:definition "Brush type; a flat, wide brush with shorter hairs, exactly the same shape as a Bright brush; ideal for creating hard edges and square fields of colour; great for street-scapes and other architectural subject matter." ;
	skos:notation "0f1c6842-17ba-4108-b843-0df01ba88a53" ;
	skos:inScheme voc:watercolorPainting ;																				
	.



voc:softEdge
	a skos:Concept ;
	skos:prefLabel "soft edge" ;
	skos:broader voc:watercolorTechnique ;
	skos:definition "Soft edges are edges that are indistinct and blurry, a fading or disappearing edge. In watercolor painting this can be achieved by painting Wet On Wet." ;
	skos:notation "7b00fce5-bbec-4a47-9021-3744bcaa25f5" ;
	skos:inScheme voc:watercolorPainting ;																				
	.


voc:spattering
	a skos:Concept ;
	skos:prefLabel "spattering" ;
	skos:broader voc:diffusingPaint ;
	skos:definition "Dipping a very coarse bristled brush (such as a toothbrush or stencil brush) in paint then running your finger or a stick across the bristles, thereby distributing minute particles of paint all over the place; resulting in a coarse airbrush/spray paint effect.As the description indicates, controlling the spatter is challenging.  The first time you try it, you'll likely paint your own face by accident." ;
	skos:notation "e2c7ea13-12f4-46bc-ae12-791bc6264f3c" ;
	skos:inScheme voc:watercolorPainting ;																				
	.


voc:stainingColors
	a skos:Concept ;
	skos:prefLabel "staining colors" ;
	skos:altfLabel "Staining" ;
	skos:broader voc:watercolorTerm ;
	skos:definition "Some watercolor pigments have smaller particles which means that they flow very smoothly and have intense color saturation, for example, the “Pthalo” colors, where others are more sedimentary producing more of a granular effect, for example viridian. Colors that absorb into the paper before the water has had a chance to evaporate; they’re difficult to lift and will leave a stain on the paper.  Not an indicator of paint quality as some pigments are inherently staining, and some are non-staining." ;
	skos:notation "3c573467-d82e-4957-8dc6-7d332c7038b4" ;
	skos:inScheme voc:watercolorPainting ;																				
	.


voc:stretching
	a skos:Concept ;
	skos:prefLabel "stretching" ;
	skos:broader voc:watercolorTerm ;
	skos:definition "Laying a sheet of watercolour paper on a rigid support and taping all sides down to the support in order to avoid buckling and warping; paper stays relatively flat while you paint (avoiding unwanted and uneven pooling) and the finished painting dries perfectly flat.Any paper of less than a 300lb weight will warp if not stretched; the amount of warp is dependent on the amount of water absorbed in the painting process.  Stretching is not necessary if you're using synthetic papers (which are not prone to warping) or if you're using a watercolor block as long as the painting is left on the block to dry." ;
	skos:notation "634bdf46-cea5-4093-98c5-64d062669fd6" ;
	skos:inScheme voc:watercolorPainting ;																				
	.


voc:tint
	a skos:Concept ;
	skos:prefLabel "tint" ;
	skos:broader voc:watercolorTechnique ;
	skos:definition "created by adding water to the original color; the more water that’s added, the weaker the intensity" ;
	skos:notation "c564e476-cd43-43bb-89cd-cad427f7f954" ;
	skos:inScheme voc:watercolorPainting ;																				
	.


voc:transparentPaint
	a skos:Concept ;
	skos:prefLabel "transparent paint" ;
	skos:broader voc:watercolorMaterial ;
	skos:definition "consists of pigment mixed with gum arabic, glycerin and a wetting agent" ;
	skos:notation "b7af93bb-3d61-471e-b4ca-d0858fa4295d" ;
	skos:inScheme voc:watercolorPainting ;																				
	.


voc:tubeColor
	a skos:Concept ;
	skos:prefLabel "tube color" ;
	skos:broader voc:watercolorMaterial ;
	skos:definition "Watercolor is available in tubes or pans, In tube form the paint is squeezed on to a Palette like toothpaste in pans the paint is in solid form and needs to be reactivated with water." ;
	skos:notation "ce8cec56-94d0-405d-8ef5-5eb5ab4a8f7b" ;
	skos:inScheme voc:watercolorPainting ;																				
	.


voc:variegatedWash
	a skos:Concept ;
	skos:prefLabel "variegated wash" ;
	skos:broader voc:wetIntoWetWash ;
	skos:definition "type of wet-into-wet wash that involves placing colors side by side and then mixing and blending them along their edges" ;
	skos:notation "bcccd3cf-2a61-49c6-a0af-75995443e2c6" ;
	skos:inScheme voc:watercolorPainting ;																				
	.


voc:veganBrushes
	a skos:Concept ;
	skos:prefLabel "vegan brushes" ;
	skos:broader voc:watercolorTool ;
	skos:definition "Vegan watercolor brushes are brushes made from synthetic fibers but have similar properties to natural hair brushes." ;
	skos:notation "a97ca567-a7c3-435c-9574-9d471757080e" ;
	skos:inScheme voc:watercolorPainting ;																				
	.


voc:washFlat
	a skos:Concept ;
	skos:prefLabel "wash flat" ;
	skos:broader voc:watercolorTechnique ;
	skos:definition "Is the technique of laying down a large area of even, consistent color." ;
	skos:notation "14d6e4e7-0c1f-4a71-8703-414f398edeb2" ;
	skos:inScheme voc:watercolorPainting ;																				
	.


voc:washVariegated
	a skos:Concept ;
	skos:prefLabel "wash variegated" ;
	skos:broader voc:watercolorTechnique ;
	skos:definition "A variegated wash is a wash painted with different colors in a wet into wet blend. Variegated washes are a signature technique of watercolor painting. They are often used to convey the natural scattering and bouncing of light and color that occurs in real life. Variegated washes can also be used to create abstract patterns and effects." ;
	skos:notation "e39a4d8e-ad06-484a-bcb9-7fc18277e226" ;
	skos:inScheme voc:watercolorPainting ;																				
	.


voc:wash
	a skos:Concept ;
	skos:prefLabel "wash" ;
	skos:broader voc:watercolorTechnique ;
	skos:definition "; A wash is a large solid area of colour, a smooth field of colour without visible brush strokes. Washes can be just one colour, or they can gradate from a light to a dark shade of a single colour, or they can graduate from one colour to another." ;
	skos:notation "e19bbd3a-1801-4941-9857-9b92046977e2" ;
	skos:inScheme voc:watercolorPainting ;																				
	.


voc:weight
	a skos:Concept ;
	skos:prefLabel "weight" ;
	skos:broader voc:watercolorTerm ;
	skos:definition "The thickness of watercolor paper is referred to as it’s weight. When measured in pounds (lbs) this refers to the weight of 500 sheets. Or it can be measured in gsm. i.e. Grams per square metre. Heavier weight paper is more expensive but is more resistant to cockling." ;
	skos:notation "fbee8c7f-8434-49cd-9ba3-9682ec6a45f8" ;
	skos:inScheme voc:watercolorPainting ;																				
	.


voc:wetIntoDryWash
	a skos:Concept ;
	skos:prefLabel "wet-into-dry wash" ;
	skos:broader voc:watercolorTechnique ;
	skos:definition "also known as a glaze or layering wash; a wash that’s applied to a dry surface" ;
	skos:notation "d3e355fe-8bd9-4f46-bf65-8697f6b9ad3c" ;
	skos:inScheme voc:watercolorPainting ;																				
	.


voc:wetIntoWetWash
	a skos:Concept ;
	skos:prefLabel "wet-into-wet wash" ;
	skos:altLabel "Wet-Into-Wet" ;
	skos:altLabel "wet-on-wet" ;
	skos:broader voc:wash ;
	skos:definition "Applying a new colour to the painting without waiting for earlier applications to dry first; colours blend together without leaving of any hard edges or sharp transitions; a technique that is only partially controllable." ;
	skos:notation "6ab2e75e-b80d-440a-b874-5f4c9e39d8f2" ;
	skos:inScheme voc:watercolorPainting ;																				
	.


voc:wetOnDry
	a skos:Concept ;
	skos:prefLabel "wet on Dry" ;
	skos:broader voc:watercolorTechnique ;
	skos:definition "This is the technique of painting wet paint on to dry paper. This creates crisp hard edged shapes." ;
	skos:notation "3961a217-955b-46e5-a9ad-f1afb3d8a8e7" ;
	skos:inScheme voc:watercolorPainting ;																				
	.


voc:WatercolorGlossaryOfTerms
	a skos:Collection ;
	skos:prefLabel "Watercolor Glossary of Terms" ;
	rdfs:seeAlso <https://www.artistsnetwork.com/art-techniques/watercolor-glossary-of-terms/> ;
	skos:member voc:analogousColors	 ,
voc:casein              ,
voc:charging            ,
voc:coldPressedPaper    ,
voc:complementaryColors ,
voc:drybrushTechnique   ,
voc:flatWash            ,
voc:watercolorGlazing             ,
voc:gradatedWash        ,
voc:granulation         ,
voc:gouache  ,
voc:hardEdge            ,
voc:hotPressedPaper     ,
voc:hue                 ,
voc:intensity           ,
voc:layering            ,
voc:liftingPaint        ,
voc:lostAndFoundEdges   ,
voc:maskingFluid        ,
voc:palette             ,
voc:paletteKnife        ,
voc:panPaint            ,
voc:pigment             ,
voc:roughPaper          ,
voc:softEdge            ,
voc:scrubbing           ,
voc:stainingColors      ,
voc:temperatureColor         ,
voc:tint                ,
voc:transparentPaint    ,
voc:value               ,
voc:variegatedWash      ,
voc:wetIntoDryWash      ,
voc:wetIntoWetWash ;
.

voc:WatercolourTerminology
	a skos:Collection ;
	skos:prefLabel "Watercolour Terminology" ;
	rdfs:seeAlso <https://cowans.org/blogs/cowans-art-knowledge-know-how/talk-like-an-artist-watercolour-terminology> ;
	skos:member voc:atomiser				,
voc:atmosphericPerspective ,
voc:backrun                ,
voc:blotting               ,
voc:bodyColour             ,
voc:buckle                 ,
voc:catsTongue            ,
voc:coldPressed            ,
voc:dryBrushing            ,
voc:fan                    ,
voc:frisket                ,
voc:watercolorGlazing                ,
voc:granulation            ,
voc:gumArabic              ,
voc:hotPressedPaper             ,
voc:impressing             ,
voc:indenting              ,
voc:liftingPaint                ,
voc:linerRigger            ,
voc:mopBrush               ,
voc:opaque                 ,
voc:overPainting           ,
voc:oxGall                 ,
voc:resist                 ,
voc:rigger                 ,
voc:sedimentary            ,
voc:scrapingDryPaint              ,
voc:shader                 ,
voc:spattering             ,
voc:sizing                 ,
voc:paintingTool           ,
voc:stainingColors               ,
voc:stipple                ,
voc:stretching             ,
voc:transparent            ,
voc:underdrawing           ,
voc:wash                   ,
voc:wetOnWet ;
.

voc:AZGlossaryOfWatercolorTerms
	a skos:Collection ;
	skos:prefLabel "A – Z Glossary Of Watercolor Terms (With Pics)" ;
	rdfs:seeAlso <https://www.solvingwatercolour.com/a-z-glossary-of-watercolor-terms-with-pics/> ;
	skos:member voc:abstract				,
voc:relatedBlogPosts        ,
voc:analogousColors         ,
voc:backrun                 ,
voc:bambooBrush             ,
voc:bead                    ,
voc:binder                  ,
voc:block                   ,
voc:bloom                   ,
voc:watercolorCanvas                  ,
voc:casein                  ,
voc:cauliflower             ,
voc:charging                ,
voc:chroma                  ,
voc:cockling                ,
voc:coldPressedPaper        ,
voc:colorWheel              ,
voc:complementaryColors     ,
voc:daggerBrush             ,
voc:deckledEdges            ,
voc:dryBrushTechnique       ,
voc:watercolorEasel                   ,
voc:fanBrush                ,
voc:flatBrush               ,
voc:watercolorGlazing                 ,
voc:gouache                 ,
voc:graduatedWash           ,
voc:granulation             ,
voc:watercolorGround                  ,
voc:gumArabic               ,
voc:hakeBrush               ,
voc:happyAccident           ,
voc:hardEdge                ,
voc:hotPressedPaper         ,
voc:hue                     ,
voc:intensity               ,
voc:kolinskySable           ,
voc:layering                ,
voc:liftingPaint              ,
voc:lineWash              ,
voc:loosePaintingStyle      ,
voc:lostFoundEdges        ,
voc:mopBrush                ,
voc:maskingFluid            ,
voc:maskingTape             ,
voc:frameMat                ,
voc:watercolorMedium                  ,
voc:mud                     ,
voc:naturalHairBrushes      ,
voc:neutralColour           ,
voc:nOTPaper                ,
voc:overworking             ,
voc:palette                 ,
voc:paletteKnife            ,
voc:pan                     ,
voc:pigment                 ,
voc:pleinAir                ,
voc:primaryColor            ,
voc:primaryColours          ,
voc:roughPaper              ,
voc:roundBrush              ,
voc:scrubbing               ,
voc:sizing                  ,
voc:softEdge                ,
voc:splitPrimariesPalette   ,
voc:stainingColors          ,
voc:stretching              ,
voc:syntheticBrushes        ,
voc:temperatureColor        ,
voc:thumbnail               ,
voc:tint                    ,
voc:tubeColor               ,
voc:value                   ,
voc:veganBrushes            ,
voc:wash                    ,
voc:washFlat                ,
voc:washVariegated          ,
voc:weight                  ,
voc:wetOnDry                ,
voc:wetIntoWetWash              ;
.

voc:AdvancedWatercolorTechniques
	a skos:Collection ;
	skos:prefLabel "Advanced Watercolor Techniques" ;
	skos:definition "Once you have mastered the basic skills of color mixing, applying washes, softening edges, dropping in color etc. there are a number of more advanced watercolor techniques you can incorporate into your work." ;
	rdfs:seeAlso <https://www.johnlovett.com/watercolor-techniques> ;
	skos:member voc:masking	,
voc:candleWaxResist				,
voc:clingWrapWash               ,
voc:draggingPaint               ,
voc:gessoUnderpainting          ,
voc:japaneseRicePaper           ,
voc:opaqueGouacheContrast,
voc:paperBlotting               ,
voc:paperMasking                ,
voc:pastelScrape                ,
voc:pressingintowetpaper        ,
voc:scrapingDryPaint            ,
voc:sprayedInk                  ,
voc:washedInk                   ,
voc:washedInkwithGouacheMask    ;
.

voc:washedInk
	a skos:Concept ;
	skos:prefLabel "washed ink" ;
	skos:broader voc:inkWash ;
	skos:definition "Waterproof ink is applied, allowed to almost dry, then scrubbed off. This will produce interesting textures and shapes. The results are unpredictable and permanent, so this technique is best used before watercolor washes are added. Best results are obtained using a spray bottle of water and rough bristle brush to scrub the ink back." ;
	skos:notation "c16d623d-f9ca-4c2d-8e61-60ab94fcfb17" ;
	.
voc:washedInkwithGouacheMask
	a skos:Concept ;
	skos:prefLabel "washed ink with gouache mask" ;
	skos:broader voc:inkWash ;
	skos:definition "For this technique, thick white gouache is painted on to preserve any areas of white paper. The gouache is allowed to thoroughly dry before being completely covered with pigment ink. When the ink is dry the surface is washed back with a water spray and bristle brush, dissolving the gouache and revealing the white paper underneath." ;
	skos:notation "e8543f32-fd38-4fa6-93f1-a7acecaf62d2" ;
	skos:inScheme voc:watercolorPainting ;																				
	.
voc:sprayedInk
	a skos:Concept ;
	skos:prefLabel "sprayed ink" ;
	skos:broader voc:diffusingPaint ;
	skos:definition "The rich colors and linear quality of permanent artists ink can be used to unify a painting. Experiment using a fine water spray just after the ink is applied. The soft spidery textures add an ancient weathered patina to your painting." ;
	skos:notation "1fdb2218-887b-4e9c-ad04-008077469ad3" ;
	skos:inScheme voc:watercolorPainting ;																				
	.
voc:candleWaxResist
	a skos:Concept ;
	skos:prefLabel "candle wax resist" ;
	skos:broader voc:assistedWash ;
	skos:definition "Wherever candle wax is applied to the painting surface, no paint will adhere. White areas can be preserved in this way before the painting is started. Unlike white preserved with masking fluid, the area can never be painted over. Washes of underlying color can be preserved in this way too. The various colored marks in the example below were preserved by drawing wax onto a dry wash then applying another wash, waiting until it drys then drawing on more wax marks." ;
	skos:notation "b2c1e858-ef89-4a38-9a67-cf19b4808af4" ;
	skos:inScheme voc:watercolorPainting ;																				
	.
voc:scrapingDryPaint
	a skos:Concept ;
	skos:prefLabel "scraping dry paint" ;
	skos:altLabel "Sgraffito" ;
	skos:broader voc:removingPaint ;
	skos:definition "Gently scraping paint off of the substrate (paper, in this case); scraping usually takes place after the paint has dried (or at least partially dried); results in subtle details and irregular textures and can help in restoring white space.  A razor blade or craft knife, sandpaper, a piece of cardboard or a cut up credit card can be used; anything scratchy." ;
	skos:notation "1ba2dbda-8bec-4fd7-b420-391aed45d52a" ;
	skos:inScheme voc:watercolorPainting ;																				
	.
voc:paperMasking
	a skos:Concept ;
	skos:prefLabel "paper masking" ;
	skos:broader voc:assistedWash ;
	skos:definition "Cartridge paper can be torn to a suitable shape, placed on the painting then the area left exposed can be wiped over with a damp brush or sponge to remove pigment. This process works best with sedimentary and non staining colors. The technique can also be used with straight edged paper to change the tone in a formal, geometric manner." ;
	skos:notation "81993099-3dc0-40fc-b5cc-43ead65e291d" ;
	skos:inScheme voc:watercolorPainting ;																				
	.
voc:pressingIntoWetPaper
	a skos:Concept ;
	skos:prefLabel "pressing into wet paper" ;
	skos:broader voc:watercolorTechnique ;
	skos:definition "This is a simple watercolor technique where a variety of objects (brush handles, empty ball point pens, blunt knives) can be used to compress the paper while a wash is still wet. The compressed paper will absorb more pigment than the surrounding paper leaving interesting dark marks in your painting.​" ;
	skos:notation "d9d7de01-01ad-45bd-985b-57bca6d9c06d" ;
	skos:inScheme voc:watercolorPainting ;																				
	.
voc:japaneseRicePaper
	a skos:Concept ;
	skos:prefLabel "Japanese rice paper" ;
	skos:broader voc:assistedWash ;
	skos:definition "Torn Japanese Rice Paper is glued to the surface with dilute PVA glue, Matt acrylic varnish  or a similar neutral pH glue.​ The results are interesting and unpredictable, depending on the type of rice paper." ;
	skos:notation "43b906f0-9585-45b0-9d2f-2606c927816b" ;
	skos:inScheme voc:watercolorPainting ;																				
	.
voc:paperBlotting
	a skos:Concept ;
	skos:prefLabel "paper blotting" ;
	skos:broader voc:liftingPaint ;
	skos:definition "Crumpled paper towel will lift pigment from a wet was in a soft, predictable way. Keep rotating and re crumpling the paper so you dont get a repeating pattern in the blot marks. This is a good watercolor technique for lifting clouds out of a wet sky.  Manually soaking up excess paint before it dries using a small sponge, piece of absorbent tissue or a towel" ;
	skos:notation "a4f31341-cee3-4542-b3aa-43bc6c9cefe7" ;
	skos:inScheme voc:watercolorPainting ;																				
	.
voc:opaqueGouacheContrast
	a skos:Concept ;
	skos:prefLabel "opaque gouache contrast" ;
	skos:broader voc:watercolorTechnique ;
	skos:definition "The contrast between transparent watercolor and flat, opaque gouache can add interest and vibrancy to a painting. Be sure to keep distinct areas of watercolor and gouache or the opaque/transparent contrast will be lost. See the article on Gouache for more information." ;
	skos:notation "5d8342fe-be68-4636-af4c-850692bdf493" ;
	skos:inScheme voc:watercolorPainting ;																				
	.
voc:gessoUnderpainting
	a skos:Concept ;
	skos:prefLabel "gesso underpainting​" ;
	skos:broader voc:watercolorTechnique ;
	skos:definition "With this watercolor technique, rough gesso brushstrokes add interest to the predictable texture of watercolor paper. Watercolor gesso or absorbent ground works best. The important thing to remember is to allow the gesso to dry thoroughly before painting on it. Watercolor, particularly sedimentary colors will settle into the fine crevasses in the gesso brush strokes making an interesting texture. " ;
	skos:notation "1ae248d0-9da9-4bd2-a241-088f0181d428" ;
	skos:inScheme voc:watercolorPainting ;																				
	.
voc:clingWrapWash
	a skos:Concept ;
	skos:prefLabel "cling wrap wash" ;
	skos:broader voc:assistedWash ;
	skos:definition "A simple technique where cling wrap is arranged over a wet wash and left until the wash is thoroughly dry. The results are fairly predictable, but this technique makes interesting rock like textures" ;
	skos:notation "f22b0010-46a7-4ec0-b412-e3e55820cd6d" ;
	skos:inScheme voc:watercolorPainting ;																				
	.
voc:pastelScrape
	a skos:Concept ;
	skos:prefLabel "pastel scrape" ;
	skos:broader voc:watercolorTechnique ;
	skos:definition "Into a wet wash scrape the dust off a suitably colored pastel with a sharp blade. Test the pastel color against a patch of the dry wash first. This technique works well with sedimentary pigments using a similar colored pastel." ;
	skos:notation "f97dbfbb-8365-4b89-8776-b2d59ca81b72" ;
	skos:inScheme voc:watercolorPainting ;																				
	.
voc:draggingPaint
	a skos:Concept ;
	skos:prefLabel "dragging paint" ;
	skos:broader voc:brushingPaint ;
	skos:definition "Dipping a paint brush handle into fresh paint and dragging it through a wet wash makes an interesting, unpredictable line ranging from soft feathered edges to solid dabs of paint" ;
	skos:notation "d3313d82-a7ee-4b29-9ec6-6e9acb13583c" ;
	skos:inScheme voc:watercolorPainting ;																				
	.

